

<section xml:id="Ch1Sec5ResultsVectorSpace">
  <title>Some results about abstract vector spaces</title>
  <p>
    It is time to use the rules of a vector space to prove some general results.
  </p>

  <assemblage>
    <p>
      We are about to do our first formal proof in the course!
    </p>
  </assemblage>

  <lemma>
    <statement>
      <p>
        Suppose <m>V</m> is a vector spaces with zero vector <m>\ve{0}</m>.
        If <m>\ve{0}'</m> is another vector satisfying R3(a) ,
        <men xml:id="uniqueness_zero">
          \ve{0}' + \ve{v} = \ve{v} \text{ for all }\ve{v} \in V
        </men>
        then <m>\ve{0} = \ve{0}'</m>.
      </p>
    </statement>
  </lemma>

  <proof>
    <md>
      <mrow>\ve{0} \amp = \ve{0}' + \ve{0} \amp \mbox{using } <xref ref="uniqueness_zero"/> \text{ with } \ve{v}=0 </mrow>
      <mrow>\amp = \ve{0}' \amp \mbox{R3(a)}   </mrow>
    </md>
  </proof>

  <definition>
    <statement>
      <p>
        If <m>V</m> is a vector space,
        we define the <term>additive inverse</term>
        of a vector <m>\ve{v} \in V</m> as
        <me>
          - \ve{v} := (-1) \cdot \ve{v}
        </me>
      </p>
    </statement>
  </definition>

  <lemma xml:id="add_inv">
    <statement>
      <p>
        If <m>V</m> is a vector space,
        then for all <m>\ve{v} \in V</m>,
        <men>
          -\ve{v} + \ve{v} = \ve{0} \mbox{ and }  \ve{v} + (-\ve{v}) = \ve{0}
        </men>.
      </p>
    </statement>
  </lemma>

  <proof>
    <md>
      <mrow>-\ve{v} + \ve{v} \amp = (-1) \cdot \ve{v} + \ve{v} \amp \amp  \mbox{(using defn of \(- \ve{v}\))}</mrow>
      <mrow>\amp = (-1) \cdot \ve{v} + 1 \cdot \ve{v} \amp \amp  \mbox{(R7)}</mrow>
      <mrow>\amp  = (-1 + 1) \cdot \ve{v} \amp \amp  \mbox{(R5)}</mrow>
      <mrow>\amp = 0 \cdot \ve{v}</mrow>
      <mrow>\amp = \ve{0} \amp \amp  \mbox{(R8)}</mrow>
    </md>
    <p>
      In addition,
      <md>
        <mrow>\ve{v} + (-\ve{v}) \amp = -\ve{v} + \ve{v} \amp \amp  \mbox{(R1)}</mrow>
        <mrow>\amp  = \ve{0} \amp \amp  \mbox{(by previous proof)}</mrow>
      </md>
    </p>
  </proof>

  <lemma>
    <statement>
      <p>
        Suppose that two vectors <m>\ve{w}</m> and <m>\ve{v}</m> in a vector space satisfy <m>\ve{w} + \ve{v} = \ve{0}</m>.
        Then <m>\ve{w} = -\ve{v}</m>.
      </p>
    </statement>
  </lemma>

  <proof>
    <md>
      <mrow>\ve{w} \amp = \ve{w} + \ve{0} \amp \amp  \mbox{(R3b)}</mrow>
      <mrow>\amp = \ve{w} + (\ve{v} + -\ve{v}) \amp \amp  \mbox{by } <xref ref="add_inv"/></mrow>
      <mrow>\amp = (\ve{w} + \ve{v}) + -\ve{v}) \amp \amp  \mbox{(R2)}</mrow>
      <mrow>\amp = \ve{0} + -\ve{v} \amp \amp  \mbox{(by assumption)}</mrow>
      <mrow>\amp = -\ve{v} \amp \amp  \mbox{(R3a)} </mrow>
    </md>.
  </proof>

  <example xml:id="explicit_solve_x">
    <statement>
      <p>
        Let us practice using the rules of a vector space to perform everyday calculations.
        For instance,
        suppose that we are trying to solve for the vector <m>\ve{x}</m> appearing in the following equation:
        <men>
          \ve{v} + 7 \cdot \ve{x} = \ve{w}
        </men>
      </p>

      <p>
        We do this using the rules as follows:
        <md>
          <mrow>\ve{v} + 7 \cdot \ve{x} \amp  = \ve{w}</mrow>
          <mrow>\therefore  -\ve{v} + (\ve{v} + 7 \cdot \ve{x}) \amp  = -\ve{v} + \ve{w} \amp \amp  \mbox{(Added \(-\ve{v}\) on left to both sides)}</mrow>
          <mrow>\therefore  (-\ve{v} + \ve{v}) + 7 \cdot \ve{x} \amp  = -\ve{v} + \ve{w} \amp \amp  \mbox{(used R2 on LHS)}</mrow>
          <mrow>\therefore  \ve{0} + 7 \cdot \ve{x} \amp  = -\ve{v} + \ve{w} \amp \amp  \mbox{(used } <xref ref="add_inv"/> \mbox{ on LHS)}</mrow>
          <mrow>\therefore  7 \cdot \ve{x} \amp  =  -\ve{v} + \ve{w} \amp \amp  \mbox{(used R3a on LHS)}</mrow>
          <mrow>\therefore  \frac{1}{7} \cdot (7 \cdot \ve{x}) \amp  = \frac{1}{7} \cdot (-\ve{v} + \ve{w}) \amp \amp  \mbox{(scalar multiplied both sides by \(\frac{1}{7}\))}</mrow>
          <mrow>\therefore  (\frac{1}{7} 7) \cdot   \ve{x} \amp  = \frac{1}{7} \cdot (-\ve{v} + \ve{w}) \amp \amp  \mbox{(used R6 on LHS)}</mrow>
          <mrow>\therefore  1 \cdot \ve{x} \amp  =  \frac{1}{7} \cdot (-\ve{v} + \ve{w})  \amp \amp  \mbox{(multiplied \(\frac{1}{7}\) with \(7\))}</mrow>
          <mrow>\therefore  \ve{x} \amp  =  \frac{1}{7} \cdot (-\ve{v} + \ve{w}) \amp \amp  \mbox{(R7)}</mrow>
        </md>
      </p>

      <p>
        As the course goes on we will leave out all these steps.
        But it is important for you to be able to reproduce them all,
        if asked to do so!
      </p>
    </statement>
  </example>

  <p>
    We will need one final lemma.
  </p>

  <lemma xml:id="dichotomy_lem">
    <statement>
      <p>
        Suppose that <m>\ve{v}</m> is a vector in a vector space <m>V</m> and that <m>k</m> is a scalar.
        Then
        <me>
          k \cdot \ve{v} = \ve{0}  \Leftrightarrow  k = 0 \mbox{ or }  \ve{v} = \ve{0}
        </me>.
      </p>
    </statement>
  </lemma>

  <proof>
    <p>
      (Proof of <m>\Leftarrow</m>).
      Suppose <m>k=0</m>.
      Then <m>k \cdot \ve{v} = 0 \cdot \ve{v} = \ve{0}</m> by R8 of a vector space.
      On the other hand, suppose <m>\ve{v} = \ve{0}</m>.
      Then <m>k \cdot \ve{v} = k \cdot \ve{0} = \ve{0}</m> by <xref ref="mult_by_zero_ex">Exercise</xref>.
    </p>

    <p>
      (Proof of <m>\Rightarrow</m>).
      Suppose <m>k \cdot \ve{v} = \ve{0}</m>.
      There are two possibilities:
      either <m>k = 0</m>, or <m>k \neq 0</m>.
      If <m>k=0</m>, then we are done.
      If <m>k \neq 0</m>,
      then <m>\frac{1}{k}</m> exists and we can multiply both sides by it:
      <md>
        <mrow>k \cdot \ve{v} \amp  = \ve{0}</mrow>
        <mrow>\therefore  \frac{1}{k} \cdot (k \cdot \ve{v})  \amp  = \frac{1}{k} \cdot \ve{0} \amp \amp  \mbox{(Multiplied both sides by \(\frac{1}{k}\))}</mrow>
        <mrow>\therefore \left(\frac{1}{k} k\right) \cdot \ve{v} \amp = \ve{0} \amp \amp  \mbox{(On the LHS, we used R6. On the RHS, we used } <xref ref="mult_by_zero_ex"/>)</mrow>
        <mrow>\therefore 1 \cdot \ve{v} \amp = \ve{0} \amp \amp  \mbox{(using \(\frac{1}{k} k = 1\))}</mrow>
        <mrow>\therefore \ve{v} \amp = \ve{0} \amp \amp  \mbox{(R7)}</mrow>
      </md>
    </p>

    <p>
      Hence in the case <m>k \neq 0</m> we must have <m>\ve{v} = \ve{0}</m>,
      which is what we wanted to show.
    </p>
  </proof>
</section>

