

<section xml:id="Ch1Sec3ExampleVectorSpace">
  <title>First example of a vector space</title>
  <introduction>
    <p>
      We were led to the definition
      (<xref ref="defnvec">Definition</xref>)
      of an abstract vector space by considering the properties of sets <m>A</m>,
      <m>B</m> and <m>C</m> in <xref ref="intro1">Section</xref>.
      Let us check, for instance,
      that <m>B</m> indeed satisfies <xref ref="defnvec">Definition</xref>.
      The others will be left as exercises.
    </p>

    <p>
      \begin{example} The set <m>B</m> is a vector space.
    </p>
  </introduction>

  <subsection>
    <title>1. Define a set <m>B</m></title>
    <p>
      We define
      <men xml:id="def_of_b">
        B := \{ (u_1, \, u_2, \, u_3) : u_1, u_2, u_3 \in \mathbb{R} \mbox{ and }  u_1 - u_2 + u_3 = 0\} 
      </men>.
    </p>
  </subsection>

  <subsection>
    <title>2. Define addition, the zero vector, and scalar multiplication</title>
    <p>
      D1.
      We define addition as follows.
      Suppose <m>\ve{u} = (u_1, \, u_2, \, u_3)</m> and
      <m>\ve{v} = (v_1, , v_2, \, v_3)</m> are elements of <m>B</m>.
      Note that in particular this means
      <m>u_1 - u_2 + u_3 = 0</m> and <m>v_1 - v_2 + v_3 = 0</m>.
      We define <m>\ve{u} + \ve{v}</m> by:
      <men xml:id="def_add_in_B">
        \ve{u} + \ve{v} := (u_1 + v_1, \, u_2 + v_2, \, u_3 + v_3)
      </men>.
    </p>

    <p>
      We need to check that this makes sense.
      We are supposed to have that
      <m>\ve{u} + \ve{v}</m> is also an element of <m>B</m>.
      We can't just write down any definition!
      To check if <m>\ve{u} + \ve{v}</m> is an element of <m>B</m>,
      we need to check if it satisfies equation <xref ref="def_of_b" />.
      Let us check:
      <md>
        <mrow>\amp (u_1 + v_1) - (u_2 + v_2) + (u_3 + v_3)</mrow>
        <mrow>\amp = (u_1 - u_2 + u_3) + (v_1 - v_2 + v_3) \amp \amp  \mbox{(this algebra step is true for ordinary numbers)}</mrow>
        <mrow>\amp = 0 + 0 \amp \amp  \mbox{(since \(\ve{u}\) and \(\ve{v}\) are in \(B\))}</mrow>
        <mrow>\amp = 0</mrow>
      </md>.
    </p>

    <p>
      Therefore, <m>\ve{u} + \ve{v}</m> is indeed an element of <m>B</m>,
      so we have written down a well-defined addition operation on <m>B</m>,
      which takes two arbitrary elements of <m>B</m> and outputs another element of <m>B</m>.
    </p>

    <p>
      D2.
      We define the zero vector <m>\ve{0} \in B</m> as
      <men xml:id="zero_vec_in_B">
        \ve{0} := (0, 0, 0)
      </men>.
    </p>

    <p>
      We need to check that this makes sense.
      Does <m>(0,0,0)</m> really belong to <m>B</m>,in other words,
      does it satisfy equation <xref ref="def_of_b" />?
      Yes, since <m>0 - 0 + 0 = 0</m>.
      So we have a well-defined zero vector.
    </p>

    <p>
      D3.
      We define scalar multiplication on <m>B</m> as follows.
      Let <m>k</m> be a real number and
      <m>\ve{u} = (u_1, \, u_2, \, u_3)</m> be an element of <m>B</m>.
      We define
      <men xml:id="s_mu_in_B">
        k \cdot \ve{u} := (ku_1, \, ku_2, \, ku_3)
      </men>.
    </p>

    <p>
      We need to check that this makes sense.
      When I multiply a multiply a vector <m>\ve{u}</m> in <m>B</m> by a scalar <m>k</m>,
      the result <m>k \cdot \ve{u}</m> is supposed to be an element of <m>B</m>.
      Does <m>(ku_1, \, ku_2, \, ku_3)</m> really belong to <m>B</m>?
      Let us check that it satisfies the defining equation <xref ref="def_of_b" />:
      <md>
        <mrow>\amp  ku_1 - ku_2 + ku_3</mrow>
        <mrow>\amp = k (u_1 - u_2 + u_3) \amp \amp  \mbox{(this algebra step is true for ordinary numbers)}</mrow>
        <mrow>\amp = k 0 \amp \amp  \mbox{(since \(\ve{u}\) is in \(B\))}</mrow>
        <mrow>\amp = 0</mrow>
      </md>.
    </p>

    <p>
      Therefore, <m>k \cdot \ve{u}</m> is indeed an element of <m>B</m>,
      so we have written down a well-defined scalar multiplication operation on <m>B</m>.
    </p>
  </subsection>

  <subsection>
    <title>3. Check that the data satisfies the rules</title>
    <p>
      We must check that our data D1, D2 and D3 satisfies the rules R1 <mdash /> R8.
      So, suppose <m>\ve{u} = (u_1, \, u_2, \,u_3)</m>,
      <m>\ve{v} = (v_1, \, v_2, \, v_3)</m> and <m>\ve{w} = (w_1, \, w_2, \, w_3)</m> are in <m>B</m>,
      and suppose that <m>k</m> and <m>l</m> are real numbers.
    </p>

    <p>
      R1.
      We check:
      <md>
        <mrow>\amp  \ve{v} + \ve{w}\tag{R1.}</mrow>
        <mrow>\amp  = (v_1 + w_1, \, v_2 + w_2, \, v_3 + w_3) \amp \amp  \mbox{(by defn of addition in \(B\))}</mrow>
        <mrow>\amp  = (w_1 + v_1, \, w_2 + v_2, \, w_3 + v_3) \amp \amp  \mbox{(because \(x + y = y + x\) is true for real numbers)}</mrow>
        <mrow>\amp = \ve{w} + \ve{v}. \amp \amp  \mbox{(by defn of addition in \(B\))}</mrow>
      </md>
    </p>

    <p>
      R2.
      We check:
      <md>
        <mrow>\amp  (\ve{u} + \ve{v}) + \ve{w}</mrow>
        <mrow>\amp = ( u_1 + v_1, \, u_2 + v_2, \, u_3 + v_3) + \ve{w} \amp \amp  \mbox{(by defn of addition in \(B\))}</mrow>
        <mrow>\amp = ( (u_1 + v_1) + w_1, \, (u_2 + v_2) + w_2, \, (u_3 + v_3) + w_3) \amp \amp  \mbox{(by defn of addition in \(B\))}</mrow>
        <mrow>\amp = ( u_1 + (v_1 + w_1), \, u_2 + (v_2 + w_2), \, u_3 + (v_3 + w_3)) \amp \amp  \mbox{(since \((x + y) + z = x + (y + z)\) is true for real numbers)}</mrow>
        <mrow>\amp = \ve{u} + (v_1 + w_1, \, v_2 + w_2, \, v_3 + w_3) \amp \amp  \mbox{(by defn of addition in \(B\))}</mrow>
        <mrow>\amp = \ve{u} + (\ve{v} + \ve{w}) \amp \amp  \mbox{(by defn of addition in \(B\))} </mrow>
      </md>.
    </p>

    <p>
      R3.
      We check:
      <md>
        <mrow>\amp \ve{0} + \ve{v}</mrow>
        <mrow>\amp = ( 0, \, 0, \, 0) + (v_1, \, v_2, \, v_3) \amp \amp  \mbox{(by defn of the zero vector in \(B\)}</mrow>
        <mrow>\amp = (0 + v_1, \, 0 + v_2, \, 0 + v_3) \amp \amp  \mbox{(by defn of addition in \(B\))}</mrow>
        <mrow>\amp = (v_1, \, v_2, \, v_3) \amp \amp  \mbox{(because \(x + 0 = x\) is true for real numbers)}</mrow>
        <mrow>\amp = \ve{v}</mrow>
      </md>.
    </p>

    <p>
      By the same reasoning, we can check that <m>\ve{v} + \ve{0} = \ve{v}</m>.
    </p>

    <p>
      R4.
      We check:
      <md>
        <mrow>\amp  k \cdot ( \ve{v + w} )</mrow>
        <mrow>\amp = k \cdot (v_1 + w_1, \, v_2 + w_2, \, v_3 + w_3) \amp \amp  \mbox{(by defn of addition in \(B\)}</mrow>
        <mrow>\amp = (k (v_1 + w_1, \, k (v_2 + w_2), \, k (v_3 + w_3) ) \amp \amp  \mbox{(by defn of scalar multipliation in \(B\))}</mrow>
        <mrow>\amp = (kv_1 + kw_1, \, kv_2 + kw_2, \, kv_3 + kw_3) \amp \amp  \mbox{(since \(k(x+y) = kx + ky\) for real numbers \(x,y\))}</mrow>
        <mrow>\amp = (kv_1, \, kv_2, \, kv_3) + (kw_1, \, kw_2,\, kw_3) \amp \amp  \mbox{(by defn of addition in \(B\))}</mrow>
        <mrow>\amp = k \cdot \ve{v} + k \cdot \ve{w} \amp \amp  \mbox{(by defn of scalar multiplication in \(B\))}</mrow>
      </md>
    </p>

    <p>
      R5.
      We check:
      <md>
        <mrow>\amp  (k + l) \cdot \ve{v}</mrow>
        <mrow>\amp = ( (k+l) v_1, \, (k+l) v_2,  \, (k+l) v_3) \amp \amp  \mbox{(by defn of scalar multiplication in \(B\))}</mrow>
        <mrow>\amp = (kv_1 + lv_1, \, kv_2 + lv_2, \, kv_3 + lv_3) \amp \amp  \mbox{(since \((k+l)x = kx + lx\) for real numbers)}</mrow>
        <mrow>\amp = (kv_1, \, kv_2, \, kv_3) + (lv_1, \, lv_2, \, lv_3) \amp \amp  \mbox{(by defn of addition in \(B\))}</mrow>
        <mrow>\amp = k \cdot \ve{v} + l \cdot \ve{v} \amp \amp  \mbox{(by defn of scalar multiplication in \(B\))}</mrow>
      </md>
    </p>

    <p>
      R6.
      We check:
      <md>
        <mrow>\amp  k \cdot (l \cdot \ve{v})</mrow>
        <mrow>\amp = k \cdot (l v_1, \, l v_2, \, lv_3) \amp \amp  \mbox{(by defn of scalar multiplication in \(B\))}</mrow>
        <mrow>\amp = (k (lv_1), \, k (lv_2), \, k (lv_3)) \amp \amp  \mbox{(by defn of scalar multiplication in \(B\))}</mrow>
        <mrow>\amp = ( (kl) v_1, \, (kl) v_2, \, (kl) v_3) \amp \amp  \mbox{(since \(k(lx) = (kl)x\) for real numbers)}</mrow>
        <mrow>\amp = (kl) \cdot \ve{v} \amp \amp  \mbox{(by defn of scalar multiplication in \(B\))} </mrow>
      </md>.
    </p>

    <p>
      R7.
      We check:
      <md>
        <mrow>1 \cdot \ve{v} \amp = (1v_1, \, 1v_2, \, 1v_3) \amp \amp  \mbox{(by defn of scalar multiplication in \(B\))}</mrow>
        <mrow>\amp = (v_1, \, v_2, \, v_3) \amp \amp  \mbox{(since \(1 x = x\) for real numbers \(x\))}</mrow>
        <mrow>\amp = \ve{v}</mrow>
      </md>.
    </p>

    <p>
      R8.
      We check:
      <md>
        <mrow>0 \cdot \ve{v} \amp = (0v_1, \, 0v_2, \, 0v_3) \amp \amp  \mbox{(by defn of scalar multiplication in \(B\))}</mrow>
        <mrow>\amp = (0, \, 0, \, 0) \amp \amp  \mbox{(since \(0 x = 0\) for real numbers}</mrow>
        <mrow>\amp = \ve{0} \amp \amp  \mbox{(by defn of the zero vector in \(B\))} </mrow>
      </md>.
    </p>

    <p>
      \end{example}
    </p>
  </subsection>
</section>

