

<section xml:id="Ch2Sec2LinearIndependence">
  <title>Linear independence</title>
  <definition xml:id="defn_of_linear_ind">
    <statement>
      <p>
        A list of vectors <m>\basis{B} = \bopen \ve{v}_1, \ve{v}_2, \ldots, \ve{v}_n \bclose</m> in a vector space <m>V</m> is called
        <term>linearly independent</term> if the equation
        <men xml:id="lin_independence_eqn">
          k_1 \ve{v}_1 + k_2 \ve{v}_2 + \cdots k_n \ve{v}_n = \ve{0}
        </men>
        has only the trivial solution <m>k_1 = k_2 = \cdots = k_n = 0</m>.
        Otherwise (if <xref ref="lin_independence_eqn"/> has a solution with at least one scalar <m>k_i \neq 0</m>) the list <m>\basis{B}</m> is called <term>linearly dependent</term>.
      </p>
    </statement>
  </definition>

  <remark xml:id="remark_about_lin_dependence"> <title>Zero vector implies linear dependence</title>
    <p>
      Suppose one of the vectors <m>\ve{v}_i</m> in the list <m>\basis{B} = \bopen \ve{v}_1, \ldots, \ve{v}_n \bclose </m> is the zero vector <m>\ve{0}</m>. Then <m>\basis{B}</m> is linearly dependent, since the equation <xref ref="lin_independence_eqn" /> has the nontrivial solution
      <me>
        0 \ve{v}_1 + \cdots + 0 \ve{v}_{i-1} + 1 \ve{v}_i + 0 \ve{v}_{i+1} + \cdots + 0 \ve{v}_n = \ve{0},
      </me>
      in other words, 
      <me>
       k_1 = 0, \ldots, k_{i-1} = 0, k_i = 1, k_{i+1} = 0, \ldots, k_n = 0.
      </me>
      So: <em>a list of linearly independent vectors never contains the zero vector!</em>
    </p>
  </remark>

  <example>
    <statement>
    <p>
      The list of vectors <m>\ve{f}_1 = (-1, \, 2)</m>,
      <m>\ve{f}_2 = (1, \,1)</m> from <xref ref="three_vectors_spanning_R2_example">Example</xref>
      is linearly independent, because the equation
      <me>
        k_1 (-1, \, 2) + k_2 (1, \, 1) = (0, \, 0)
      </me>
      is equivalent to the system of equations
      <men xml:id="system_from_r2_example">
       -k_1 + k_2 = 0, \quad 2k_1 + k_2 = 0
      </men>
      which has only the trivial solution <m>k_1 = 0</m> and <m>k_2 = 0</m>.
    </p>


    </statement>
  </example>

   <exercise>
      <statement>
        <p>
          Check that <xref ref="system_from_r2_example" /> has only the trivial solution.
        </p>
      </statement>
    </exercise>

  <example xml:id="example_about_lin_dep_1">
    <statement>
    <p>
      The list of vectors <m>\ve{f}_1 = (-1, \, 2)</m>,
      <m>\ve{f}_2 = (1, \,1)</m>,
      <m>\ve{f}_3 = (2, \, -1)</m> from <xref ref="three_vectors_spanning_R2_example">Example</xref>
      is linearly dependent, because the equation
      <men xml:id="eqn_to_check_lin_ind">
        k_1 (-1, \, 2) + k_2 (1, \, 1) + k_3 (2, \, -1) = (0, \, 0)
      </men>
      is equivalent to the system of equations
      <men xml:id="system_from_r2_example_new">
       -k_1 + k_2 + 2k_3 = 0, \quad 2k_1 + k_2 - k_3 = 0
      </men>
      which has a one-dimensional vector space of solutions parameterized by <m>t</m>,
      <men xml:id="supposed_soln">
        k_1 = t, \, k_2 = -t, \, k_3 = t,  t \in \mathbb{R}
      </men>.
    </p>

    <p>
      For instance, for <m>t=2</m>, we have
      <me>
        2 (-1, \, 2) - 2 (1, \, 1) + 2 (2, \, -1) = (0, \, 0)
      </me>
      so that <xref ref="eqn_to_check_lin_ind" /> has nontrivial solutions.
    </p>
    </statement>
  </example>

    <exercise>
      <statement>
        <p>
          Check that <xref ref="system_from_r2_example_new" /> has the solution set <xref ref="supposed_soln" />.
        </p>
      </statement>
    </exercise>

  <example xml:id="new_basis_for_poly_3">
    <statement>
      <p>
        The list of polynomials
        <me>
          \ve{q}_0(x) := 1, \,\, \ve{q}_1(x) := x, \,\, \ve{q}_2(x) := 2x^2 - 1, \,\, \ve{q}_3(x) := 4x^3 - 3x
        </me>
        from <xref ref="chebyshev_example">Example</xref>
        is linearly independent in <m>\Poly_3</m>.
        This is because the equation
        <me>
          k_0 \ve{q}_0 + k_1 \ve{q}_1 + k_2 \ve{q}_2 + k_3 \ve{q}_3 = \ve{0}
        </me>
        becomes the following equation between polynomials:
        <me>
          4k_3 x^3 + 2k_2 x^2 + (-3k_3 + k_1) x + (-k_2 + k_0) = 0
        </me>
      </p>

      <p>
        This is equivalent to the following system of equations,
        <me>
          4k_3 = 0, \quad 2k_2 = 0, \quad -3 k_3 + k_1 = 0, \quad k_0 - k_2 = 0
        </me>
        which has only the trivial solution <m>k_0 = k_1 = k_2 = k_3 = 0</m>.
      </p>
    </statement>
  </example>

  <p>
    Here are two more ways to think about linearly dependent lists of vectors. 
  </p>

  <proposition xml:id="lin_dependence_prop">
    <title>Equivalent Criterions for Linear Dependence</title>
    <statement>
      <p>
        Let <m>\basis{B} = \bopen \ve{v}_1, \ldots, \ve{v}_n \bclose</m> be a list of vectors in a vector space <m>V</m>.
        The following statements are equivalent:
        <ol>
          <li xml:id="defn_lin_dep"> The list of vectors <m>\basis{B}</m> is linearly dependent. 
          </li>

          <li xml:id="lin_comb_other_vec"> 
            <emph>(Linear Combination of Other Vectors)</emph>
            <p> One of the vectors in the list <m>\basis{B}</m> is a linear combination of the other vectors in <m>\basis{B}</m>.
            </p>
          </li>

          <li xml:id="lin_comb_prec_vec"> <emph>(Linear Combination of Preceding Vectors)</emph><title>Linear Combination of Preceding Vectors</title>
            <p>
              Either <m>\ve{v}_1 = \ve{0}</m>,
              or for some <m>r \in \{2, 3, \ldots,
              n\}</m>, <m>\ve{v}_r</m> is a linear combination of <m>\ve{v}_1</m>,
              <m>\ve{v}_2</m>, <m>\ldots</m>, <m>\ve{v}_{r-1}</m>.
            </p>
          </li>
        </ol>
      </p>
    </statement>
  </proposition>

  <proof> <p>We will show that (1) <m>\Leftrightarrow</m> (2), (1) <m>\Rightarrow</m> (3) and (3) <m>\Rightarrow</m> (2), and conclude that each statement implies the others.</p>

      <p> (1) <m>\Rightarrow</m> (2). Suppose that <m>\basis{B}</m> is linearly dependent. This means that there are scalars <m>k_1</m>,
      <m>k_2</m>, <m>\ldots</m>, <m>k_n</m>, not all zero, such that
      <men xml:id="lin_dep_lem_another_eqn">
        k_1 \ve{v}_1 + k_2 \ve{v}_2 + \cdots + k_n \ve{v}_n = \ve{0}
      </men>.
      Let <m>k_s</m> be one of the nonzero coefficients. Then, by taking the other vectors to the other side of the equation, and multuplying by <m>\frac{1}{k_s}</m> we can solve for <m>\ve{v}_s</m> in terms of the other vectors:
      <md>
        <mrow>
        \ve{v}_s \amp = -\frac{k_1}{k_s} \ve{v}_1 - \ldots - \frac{k_n}{k_s} \ve{v}_n \amp \amp \mbox{(No } \ve{v}_i \mbox{ terms on RHS)}
      </mrow>
    </md>
    Therefore, (2) is true.
    </p>

    <p> (2) <m>\Rightarrow</m> (1). Suppose that one of the vectors in the list, say <m>\ve{v}_s</m>, is a linear combination of the others vectors. That is, 
    <md>
      <mrow> \ve{v}_s \amp= k_1\ve{v}_1 + \ldots + k_n \ve{v}_n \amp \amp \mbox{(No }<m>\ve{v}_s</m> \mbox{term on RHS.)} </mrow>
    </md>
    Rearranging this equation gives:
    <men xml:id="rearranged_lin_dep">
      k_1 \ve{v}_1 + \ldots + (-1)\ve{v}_s + \ldots + k_n \ve{v}_n = \ve{0}.
    </men>
    Not all the coefficients on the LHS of <xref ref="rearranged_lin_dep"/> are zero, since the coefficient of <m>\ve{v}_s</m> is equal to <m>-1</m>. Therefore, <m>\basis{B}</m> is linearly dependent.
  </p>

      <p> (1) <m>\Rightarrow</m> (3).
      Suppose that the list <m>\basis{B} = \bopen \ve{v}_1, \ldots, \ve{v}_n \bclose</m> is linearly dependent.
      This means that there are scalars <m>k_1</m>,
      <m>k_2</m>, <m>\ldots</m>, <m>k_n</m>, not all zero, such that
      <men xml:id="lin_dep_lem_first_eqn">
        k_1 \ve{v}_1 + k_2 \ve{v}_2 + \cdots + k_n \ve{v}_n = \ve{0}
      </men>.
    </p>

    <p>
      Let <m>r \in \{1, \,2, \ldots, \, n\}</m> be the largest index such that <m>k_r \neq 0</m>.
      (We are told that not all the <m>k_i</m> are zero, so this makes sense.)
      If <m>r=1</m>,
      then <xref ref="lin_dep_lem_first_eqn" /> is simply the equation
      <me>
        k_1 \ve{v}_1 = \ve{0},  \mbox{where }  k_1 \neq 0
      </me>.
    </p>

    <p>
      Therefore <m>\ve{v}_1 = \ve{0}</m> by <xref ref="dichotomy_lem">Lemma</xref>,
      and we are done.
      On the other hand, suppose <m>r \neq 1</m>.
      Then <xref ref="lin_dep_lem_first_eqn" /> becomes the equation
      <me>
        k_1 \ve{v}_1 + k_2 \ve{v}_2 + \cdots + k_r \ve{v}_r = \ve{0},  \mbox{where }  k_r \neq 0
      </me>.
    </p>

    <p>
      By dividing by <m>k_r</m>,
      we can now solve for <m>\ve{v}_r</m> in terms of the preceding vectors <m>\ve{v}_1</m>,
      <m>\ve{v}_2</m>, <m>\ldots</m>, <m>\ve{v}_{r-1}</m>:
      <me>
        \therefore \ve{v}_r = - \frac{k_1}{k_r} \ve{v}_1 - \frac{k_2}{k_r} \ve{v}_2 - \cdots - \frac{k_{r-1}}{k_r} \ve{v}_{r-1} \,
      </me>
      Therefore, (3) is true.
    </p>

     <p> (3) <m>\Rightarrow</m> (2) Suppose that (3) is true. In other words, either:
        <ul>
          <li> <m>\ve{v}_1 = \ve{0}</m>. Therefore, <m>\basis{B}</m> is linearly dependent, by <xref ref="remark_about_lin_dependence"/>. In other words, (1) is true. Therefore, since we have already proved that (1) <m>\Rightarrow </m> (2), we conclude that (2) is true. </li>
          <li> For some <m>r \in \{2, \ldots, n\}</m>, <m>\ve{v}_r</m> is a linear combination of <m>\ve{v}_1, \ldots, \ve{v}_{r-1}</m>. In this case, clearly <m>\ve{v}_r</m> is a linear combination of the other vectors in <m>\basis{B}</m>, so (2) is true.</li>
        </ul>
        In both cases, (2) is true. So, (3) <m>\Rightarrow</m> (2).
    </p>
  </proof>

  <example xml:id="app_of_prop_preceding">
    <statement>
      <p>
        We saw in <xref ref="example_about_lin_dep_1">Example</xref>, using the definition of linear dependence,
        that the list of vectors <m>\ve{f}_1 = (-1, \, 2)</m>,
        <m>\ve{f}_2 = (1, \,1)</m>,
        <m>\ve{f}_3 = (2, \, -1)</m> in
        <m>\mathbb{R}^3</m> is linearly dependent. Give two alternative proofs of this, using <xref ref="lin_dependence_prop"/>.
      </p>
    </statement>

    <solution>
      <p>We check <xref ref="lin_comb_other_vec"/> of <xref ref="lin_dependence_prop"/>. That is, we check if one of the vectors in the list is a linear combination of the other vectors. Indeed, we observe by inspection that
      <men>
       \ve{f}_2 = \ve{f}_1 + \ve{f}_3.
     </men>
     Hence, <m>\basis{B}</m> is linearly dependent.
   </p>
    </solution>


    <solution>
      <p>We check <xref ref="lin_comb_prec_vec"/> of <xref ref="lin_dependence_prop"/>. That is, we check:
        <ul>
          <li>
            <p>
              Is <m>\ve{f}_1 = \ve{0}</m>? No.
            </p>
          </li>

          <li>
            <p>Is <m>\ve{f}_2</m> is a scalar multiple of <m>\ve{f}_1</m>? No.
            </p>
          </li>

          <li>
            <p>Is
              <m>\ve{f}_3</m> is a linear combination of
              <m>\ve{f}_1</m> and <m>\ve{f}_2</m>? Yes, since
              <me>
                \ve{f}_3 = - \ve{f}_1 + \ve{f}_2.
              </me>
              Hence, <m>\basis{B}</m> is linearly dependent.
            </p>
          </li>
        </ul>
      </p>
    </solution>
  </example>

  <proposition xml:id="bumping_off_lemma">
    <title>Bumping Off Proposition</title>
    <statement>
      <p>
        Suppose <m>\basis{L} = \left\{ \ve{l}_1, \ve{l}_2, \ldots, \ve{l}_m \right\}</m> is a linearly independent list of vectors in a vector space <m>V</m>,
        and that <m>\basis{S} = \left\{ \ve{s}_1, \ve{s}_2, \ldots, \ve{s}_n \right\}</m> spans <m>V</m>.
        Then <m>m \leq n</m>.
      </p>
    </statement>
  </proposition>

  <proof>
    <p>
      Start with the original spanning list of vectors
      <men>
        \basis{S} = \left\{ \,\,  \ve{s}_1, \ve{s}_2, \ldots, \ve{s}_n \right\}
      </men>
      and consider the <sq>bloated</sq> list
      <men xml:id="bloated_list">
        \basis{S}' = \left\{\ve{l}_1, \ve{s}_1, \ve{s}_2, \cdots, \ve{s}_n \right\}
      </men>
    </p>

    <p>
      Now, since <m>\basis{S}</m> spans <m>V</m>, we know that <m>\ve{l}_1</m> can be written as a linear combination of the vectors <m>\ve{s}_1, \ldots, \ve{s}_n</m>. Therefore, by <xref ref="lin_comb_other_vec"/> of <xref ref="lin_dependence_prop"/>, we know that <m>\basis{S}'</m> is linearly dependent. Thus, by <xref ref="lin_comb_prec_vec"/> of <xref ref="lin_dependence_prop"/>, either:</p>
      <ul>
        <li> <m>\ve{l}_1 = \ve{0}</m>. This cannot be true, since then <m>\basis{L}</m> would be linearly dependent by <xref ref="remark_about_lin_dependence"/>, contradicting our initial assumption. </li>
        <li> or one of the <m>\ve{s}</m>-vectors, say <m>\ve{s}_r</m>, can be expressed as a linear combination of the preceding vectors. We can then remove <m>\ve{s}_r</m> from the list <m>\basis{S}'</m> (<sq>bump it off</sq>), and the resulting list
      <men>
        \basis{S}_1 :=  \left\{\ve{l}_1, \ve{s}_1, \ve{s}_2, \cdots, \hat{\ve{s}_r}, \cdots, \ve{s}_n \right\} \qquad \mbox{(\(\ve{s}_r\) omitted)}
      </men>
      will still span <m>V</m>, by <xref provisional="exercise-span-omission"/>. </li>
    </ul>
    <p> We can go on in this way,
      each time transferring another one of the <m>\ve{l}</m>-vectors into the list,
      and removing another one of the <m>\ve{s}</m>-vectors, and still have a list which spans <m>V</m>:
      <md>
        <mrow> 
        \basis{L} \amp = \bopen \ve{l}_1, \ldots, \ve{l}_m \bclose \amp \basis{S} \amp = \bopen \ve{s}_1, \ldots, \ve{s}_n \bclose 
      </mrow>
      <mrow>
        \basis{L}_1 \amp = \bopen \ve{l}_2, \ldots, \ve{l}_m \bclose \amp \basis{S}_1 \amp = \bopen \ve{l}_1, \underbrace{\ve{s}_1, \ldots, \ve{s}_n}_{n-1} \bclose </mrow>
      <mrow>
        \basis{L}_2 \amp = \bopen \ve{l}_3, \ldots, \ve{l}_m \bclose \amp \basis{S}_2 \amp = \bopen \ve{l}_2, \ve{l}_1, \underbrace{\ve{s}_1, \ldots, \ve{s}_n}_{n-2} \bclose </mrow>
      <mrow> \amp \vdots \amp \amp \vdots </mrow>
      </md>
    </p>
    <p>
      Now, suppose that <m>m > n</m>. When we reach the <m>n</m>th stage of this process, we will have <m>\basis{S}_n = \bopen \ve{l}_n, \ldots, \ve{l}_1 \bclose</m>, and it will span <m>V</m>. Therefore, in particular, <m>\ve{l}_{n+1}</m> (which we know exists, since <m>m > n </m>) will be a linear combination of <m>\ve{l}_1, \ldots, \ve{l}_n</m>. But then, by <xref ref="lin_comb_other_vec"/> of <xref ref="lin_dependence_prop"/>, we conclude that <m>\basis{L}</m> is linearly dependent. But we were told in the beginning that <m>\basis{L}</m> is linearly indepedent, so we have a contradiction. Hence, our assumption that <m>m > n</m> must be false. Therefore, we must have <m>m \leq n</m>. 
   </p>
  </proof>

  <exercises>
  <exercise>
    <statement>
      <p>
        Show that the list of vectors
        <m>(2, \, 3, \, 1)</m>, <m>(1, \, -1, \, 2)</m>,
        <m>(7, \, 3, \, c)</m> is linearly dependent in
        <m>\mathbb{R}^3</m> if and only if <m>c=8</m>.
      </p>
    </statement>
  </exercise>

  <exercise xml:id="x2_by_2_matrices_lin_dep">
    <statement>
      <p>
        The list of vectors in <m>\Mat_{2,2}</m> given by
         <me>
\ve{v}_1 = \begin{bmatrix}
1 &amp; 2 \\
1 &amp; 1
\end{bmatrix},\,
\ve{v}_2 = \begin{bmatrix}
1 &amp; 0 \\
-2 &amp; 1
\end{bmatrix},\,
\ve{v}_3 = \begin{bmatrix}
1 &amp; 0 \\
2 &amp; 3
\end{bmatrix},\,
\ve{v}_4 = \begin{bmatrix}
0 &amp; 3 \\
1 &amp; -1
\end{bmatrix},\,
\ve{v}_5 = \begin{bmatrix}
1 &amp; 0 \\
0 &amp; 1
\end{bmatrix}
      </me>
        is linearly independent
        (you will prove this in <xref ref="checking_matrices_lin_dep">Exercise</xref>,
        but for the sake of this question you may assume it to be true).
        Go through the same steps as in <xref ref="app_of_prop_preceding">Example</xref>
        to find the first vector in the list which is either the zero vector or a linear combination of the preceding vectors.
      </p>
    </statement>
  </exercise>

  <exercise xml:id="exercise-span-omission">
    <statement> Let <m>\basis{S} = \bopen \ve{v}_1, \ldots, \ve{v}_n \bclose </m> be a list of vectors in a vector space <m>V</m>. Suppose that <m>\basis{S}</m> spans <m>V</m>. Suppose that <m>w</m> is another vector in <m>V</m>. Prove that the list of vectors <m>\basis{S}' = \bopen \ve{w}, \ve{v}_1, \ldots, \ve{v}_n \bclose</m> also spans <m>V</m>.
    </statement>
  </exercise>

  </exercises>
</section>

